almost there...

monad/smonad2.v
@@ -5,16 +5,23 @@ Variable ST : Set.
 
 Definition CS_Pre : Type
   := ST -> Prop.
+Hint Unfold CS_Pre.
+
 Definition CS_Post (A:Set) : Type :=
   ST -> A -> nat -> ST -> Prop.
+Hint Unfold CS_Post.
+
+Definition CS_Arg (pre : CS_Pre) := { st : ST | pre st }.
+Hint Unfold CS_Arg.
 
 Program Definition
   CS (pre : CS_Pre) (A : Set) (post : CS_Post A) : Set :=
-  forall st : { st : ST | pre st },
+  forall st : (CS_Arg pre),
     { (a, st') : A * ST | exists an, post st a an st' }.
 Hint Unfold CS.
 
 Definition top : CS_Pre := fun st => True.
+Hint Unfold top.
 
 Program Definition ret (A : Set) (post : CS_Post A) 
   : forall av,
@@ -31,43 +38,53 @@ Defined.
 Program Definition bind:
   forall (A:Set)
     (preA : CS_Pre) (postA : CS_Post A) (am:(CS preA A postA))
-    (B:Set) (preB : A -> CS_Pre) (postB : A -> CS_Post B)
-    (bf:(forall (a : A)
-      (posta:exists st0 an stA,
-        postA st0 a an stA),
-      (CS (preB a) B
-        (fun stA b bn stB =>
-          forall st0 an,
-            postA st0 a an stA ->
-            postB a stA b (an+bn) stB)))),
+    (B:Set) (preB : A -> nat -> CS_Pre) (postB : A -> CS_Post B)
+    (bf:(forall (a : A),
+      (CS
+        (fun stA =>
+          exists st an,
+            postA st a an stA /\
+            preB a an stA)
+        B
+        (fun stA bv bn stB =>
+          forall an,
+            preB a an stA ->
+            postB a stA bv (an+bn) stB)))),
     CS (fun st0 =>
       preA st0 /\
       (forall a an stA,
         postA st0 a an stA ->
-        preB a stA))
+        preB a an stA))
     B
     (fun st0 b bn stB =>
       exists a an stA,
         postA st0 a an stA /\
-        postB a stA b bn stB).
+        postB a stA b (an+bn) stB).
 Proof.
   intros.
   intros [st0 [preA_st0 postApreB]].
   edestruct (am (exist preA st0 preA_st0))
    as [[av stA] postA_stA].
-  simpl in postA_stA.
-  assert (preB av stA) as preB_stA.
-  destruct postA_stA. eauto. simpl.
-  assert (exists (st0 : ST) (an : nat) (stA : ST), postA st0 av an stA) as postav.
-  destruct postA_stA. exists st0. exists x. exists stA. auto.
-  edestruct (bf av postav (exist (preB av) stA preB_stA)) as
-    [[bv stB] postApostB_stB].
-  simpl in postApostB_stB.
+  simpl in *.
+
+  assert ((fun stA : ST =>
+    exists (st : ST) (an : nat), postA st av an stA /\ preB av an stA)
+  stA) as preB_stA.
+  destruct postA_stA as [an postA_stA]. eauto. 
+  
+  edestruct
+  (bf av (exist (fun stA : ST =>
+    exists (st : ST) (an : nat), postA st av an stA /\ preB av an stA) stA preB_stA))
+  as [[bv stB] postApostB_stB].
   exists (bv, stB).
-  simpl.
   destruct postA_stA as [an postA_stA].
-  destruct postApostB_stB as [bn postApostB_stB].
-  exists (an + bn). exists av. exists an. eauto. 
+  destruct postApostB_stB as [bn postB_stB].
+  simpl in *.
+  exists bn. exists av.
+  exists an. exists stA.
+  split. auto.
+  eapply postB_stB.
+  eauto.
 Defined.
 
 Program Definition get:
@@ -132,40 +149,52 @@ Program Fixpoint list_insert x (l:list nat) :
         (fun st r ln st' => r = bare_list_insert x l /\ ln = length l /\ st' = st)
         (cons x nil) _)
     | cons y sl =>
-      (@bind ST (list nat)
+      (@bind ST
+        (list nat)
         (fun st => True)
         (fun st r ln st' => r = bare_list_insert x sl /\ ln = length sl /\ st' = st)
         (list_insert x sl)
+        
         (list nat)
-        (fun sl' st => sl' = bare_list_insert x sl)
+        (fun sl' sl'n st => sl'n = length sl /\ sl' = bare_list_insert x sl)
         (fun sl' st r ln st' => r = bare_list_insert x l /\ ln = length l /\ st' = st)
-        (fun sl' postsl' =>
+        (fun sl' =>
           (@inc ST 1 (fun st => True) (list nat)
-            (fun st r ln st' => r = bare_list_insert x l /\ ln = length l /\ st' = st)
+            (fun st r ln st' => r = (cons y sl') /\ ln = 1 /\ st' = st)
             (@ret ST (list nat)
-              (fun st r ln st' => r = bare_list_insert x l /\ ln = 0 /\ st' = st)
+              (fun st r ln st' => r = (cons y sl') /\ ln = 0 /\ st' = st)
               (cons y sl') _))))
   end.
 
 Next Obligation.
+  rename x0 into st.
+  destruct st as [st Pre_st].
   simpl. eauto.
 Defined.
 
 Next Obligation.
   simpl.
   rename x0 into st.
-  rename H1 into Pre_st.
-  exists (length sl). intros.
-  split. auto. split. omega. auto.
+  destruct st as [st Pre_st].
+  simpl.
+  exists 0.
+  intros am. simpl.
+  intros EQ. subst am.
+  auto.
 Defined.
 
 Next Obligation.
-  simpl.
   rename x0 into st.
-  rename H4 into Pre_st.
+  destruct st as [st Pre_st].
+  simpl in *.
+  destruct Pre_st as [st' [sl'n [[EQ1 [EQ2 EQ3]] [EQ4 EQ5]]]].
+  subst sl'. subst st'. subst sl'n.
   exists 1.
-  intros st0 an [EQr [EQln EQst]].
-  split. auto. split. omega. auto.
+  intros an.
+  intros [EQ1 EQ2].
+  subst an.
+  repeat split; auto.
+  omega.
 Defined.
 
 Next Obligation.
@@ -173,14 +202,8 @@ Next Obligation.
 Defined.
 
 Next Obligation.
-  simpl.
-  rename x0 into st.
-  rename H into ST_Pre_st.
-  destruct (list_insert x sl (exist (fun _ : ST => True) st I)) as [[sl' st'] IH].
-  destruct IH as [sl'n [EQsl' [EQsl'n EQst]]].
-  simpl in *.
-  subst st' sl' sl'n.
-  eauto.
+  exists (S (length sl)).
+  auto.
 Defined.
 
 Program Definition insert (x:nat) :
@@ -197,10 +220,10 @@ Program Definition insert (x:nat) :
   (@get ST)
 
   ()
-  (fun av st => st = av)
+  (fun av an st => an = 0 /\ st = av)
   (fun av st _ bn st' =>
     st = av /\ bn = length st /\ st' = bare_list_insert x st)
-  (fun l postl =>
+  (fun l =>
     (@bind ST
 
       ST 
@@ -210,20 +233,31 @@ Program Definition insert (x:nat) :
       (list_insert x l)
       
       ()
-      (fun l' st => l' = bare_list_insert x st)
+      (fun l' l'n st =>  l'n = length st /\ l' = bare_list_insert x st)
       (fun l' st _ bn st' =>
         l' = bare_list_insert x st /\ bn = length st /\ st' = l')
-      (fun l' postl' =>
+      (fun l' =>
         (@put ST l')))).
 
 Next Obligation.
+  rename x0 into st.
+  destruct st as [st Pre_st].
   simpl. eauto.
 Defined.
 
 Next Obligation.
-  destruct (list_insert x postl (exist (fun _ : ST => True) postl I))
+  rename x0 into st.
+  destruct st as [st Pre_st].
+  simpl.
+
+  destruct (list_insert x l
+          (exist (fun _ : ST => True) st
+             (insert_obligation_2 x l
+                (exist (fun st0 : ST => st0 = l) st Pre_st))))
     as [[a st'] [an [EQa [EQan EQst']]]].
   simpl in *.
+  subst a an st' st.
+  exists (length l).
   eauto.
 Defined.
 
@@ -232,414 +266,75 @@ Next Obligation.
 Defined.
 
 Next Obligation.
-  eexists. intros st0 an.
-  intros [EQr [EQan EQst]].
-  subst an x0. eauto.
+  rename x0 into st.
+  destruct st as [st [st' [an [[EQl' [EQan EQst']] [EQan2 EQl'2]]]]].
+  subst l' an st'.
+  simpl.
+  exists 0. intros an [EQan EQl].
+  subst an. auto.
 Defined.
 
 Next Obligation.
-  split; auto.
-  intros a an stA [EQa [EQan EQst]].
+  rename x0 into st.
+  destruct st as [st [st' [an [[EQl [EQan stA]] [EQan2 EQstA]]]]].
+  simpl. subst st' an st.
+  split; auto. clear EQan2 stA.
+  intros a an stA [EQa [EQan EQstA]].
   subst a an stA.
   auto.
 Defined.
 
-(* XXX This "proof" is insane. What does it mean? *)
 Next Obligation.
-  program_simpl.
-  edestruct (list_insert x postl _).
-  
-  destruct (insert_obligation_6 x postl
-           (ex_intro
-              (fun st0 : ST =>
-               exists (an : nat) (stA : ST),
-                 postl = st0 /\ an = 0 /\ stA = st0) postl
-              (ex_intro
-                 (fun an : nat =>
-                  exists stA : ST, postl = postl /\ an = 0 /\ stA = postl) 0
-                 (ex_intro
-                    (fun stA : ST => postl = postl /\ 0 = 0 /\ stA = postl)
-                    postl (conj eq_refl (conj eq_refl eq_refl)))))
-           (exist (fun st : ST => st = postl) postl eq_refl)).
+  rename x0 into st.
+  destruct st as [st Pre_st].
+  simpl.
+  destruct Pre_st as [st' [an [[EQl [EQan EQst]] [EQan2 EQst2]]]].
+  subst st' an st. simpl.
+  clear EQan2.
+  destruct (list_insert x l
+                (exist (fun _ : ST => True) l
+                   (insert_obligation_2 x l
+                     (exist (fun st : ST => st = l) l EQst))))
+  as [[l' st'] [an [EQl' [EQan EQst']]]].
   simpl in *.
-  remember (insert_obligation_3 x postl
-             (ex_intro
-                (fun st0 : ST =>
-                 exists (an : nat) (stA : ST),
-                   postl = st0 /\ an = 0 /\ stA = st0) postl
-                (ex_intro
-                   (fun an : nat =>
-                    exists stA : ST, postl = postl /\ an = 0 /\ stA = postl)
-                   0
-                   (ex_intro
-                      (fun stA : ST => postl = postl /\ 0 = 0 /\ stA = postl)
-                      postl (conj eq_refl (conj eq_refl eq_refl)))))
-             (exist (fun st : ST => st = postl) postl e)).
-  simpl in *.
-  clear Heqy.
-  destruct (list_insert x postl (exist (fun _ : ST => True) postl I)).
-  simpl in *.
-  destruct x0 as [a st]. simpl in *.
-  exists (length postl).
-  intros st0 an [EQp [EQan EQp2]].
-  subst.
-  repeat split; eauto.
-  destruct y. intuition.
-Qed.
+  subst l' an st'. clear EQst.
+  exists (length l).
+  intros an [EQan EQl].
+  subst an. simpl. auto.
+Defined.
 
 Next Obligation.
-  intuition. subst. auto.
-Qed.
+  rename x0 into st.
+  destruct st as [st Pre_st].
+  split; auto.
+  intros a an stA. simpl.
+  intros [EQa [EQan EQstA]].
+  subst. auto.
+Defined.
 
 Next Obligation.
-  rename x0 into st0.
-  rename H into preA.
-  destruct (insert_obligation_8 x (exist (fun _ : ST => True) st0 preA))
-    as [preA_st0 postApreB].
+  rename x0 into st.
+  destruct st as [st Pre_st].
   simpl in *.
-  clear preA.
-  destruct (insert_obligation_1 x (exist (fun _ : ST => True) st0 preA_st0))
-    as [an postA_stA].
-  simpl in *.
-  clear preA_st0.
-  destruct postA_stA as [E0 [E1 E2]].
-  subst an.
-  
-  clear postApreB.
-  
-  
-  remember (insert_obligation_7 x x0
-             match
-               insert_obligation_1 x (exist (fun _ : ST => True) x0 preA_st0)
-             with
-             | ex_intro x1 H0 =>
-                 ex_intro
-                   (fun st0 : ST =>
-                    exists (an : nat) (stA : ST),
-                      x0 = st0 /\ an = 0 /\ stA = st0) x0
-                   (ex_intro
-                      (fun an : nat =>
-                       exists stA : ST, x0 = x0 /\ an = 0 /\ stA = x0) x1
-                      (ex_intro
-                         (fun stA : ST => x0 = x0 /\ x1 = 0 /\ stA = x0) x0
-                         H0))
-             end
-             (exist (fun st : ST => st = x0) x0
-                match
-                  insert_obligation_1 x
-                    (exist (fun _ : ST => True) x0 preA_st0)
-                with
-                | ex_intro x1 H0 => postApreB x0 x1 x0 H0
-                end)).
-  simpl in *.
-  rewrite <- Heqy.
-  clear Heqy.
 
-  
-  destruct ((let (bv, stB) as p
-             return
-               ((let (_, st') := p in
-                 exists an : nat,
-                   forall (st0 : ST) (an0 : nat),
-                   x0 = st0 /\ an0 = 0 /\ x0 = st0 ->
-                   x0 = x0 /\
-                   an0 + an = length x0 /\ st' = bare_list_insert x x0) ->
-                { (_, st') : () * ST |
-                exists (an : nat) (a0 : ST) (an0 : nat) 
-                (stA : ST),
-                  (a0 = x0 /\ an0 = 0 /\ stA = x0) /\
-                  stA = a0 /\ an = length stA /\ st' = bare_list_insert x stA}) :=
-             `
-             match
-               insert_obligation_6 x x0
-                 match
-                   insert_obligation_1 x
-                     (exist (fun _ : ST => True) x0 preA_st0)
-                 with
-                 | ex_intro x1 H0 =>
-                     ex_intro
-                       (fun st0 : ST =>
-                        exists (an : nat) (stA : ST),
-                          x0 = st0 /\ an = 0 /\ stA = st0) x0
-                       (ex_intro
-                          (fun an : nat =>
-                           exists stA : ST, x0 = x0 /\ an = 0 /\ stA = x0) x1
-                          (ex_intro
-                             (fun stA : ST => x0 = x0 /\ x1 = 0 /\ stA = x0)
-                             x0 H0))
-                 end
-                 (exist (fun st : ST => st = x0) x0
-                    match
-                      insert_obligation_1 x
-                        (exist (fun _ : ST => True) x0 preA_st0)
-                    with
-                    | ex_intro x1 H0 => postApreB x0 x1 x0 H0
-                    end)
-             with
-             | conj preA_st1 postApreB0 =>
-                 (let (av, stA) as p
-                      return
-                        ((let (a, st') := p in
-                          exists an : nat,
-                            a = bare_list_insert x x0 /\
-                            an = length x0 /\ st' = x0) ->
-                         { (_, st') : () * ST |
-                         exists (an : nat) (a0 : ST) 
-                         (an0 : nat) (stA : ST),
-                           (a0 = bare_list_insert x x0 /\
-                            an0 = length x0 /\ stA = x0) /\
-                           a0 = bare_list_insert x stA /\
-                           an = length stA /\ st' = a0}) :=
-                      `
-                      (list_insert x x0
-                         (exist (fun _ : ST => True) x0
-                            (insert_obligation_2 x x0
-                               match
-                                 insert_obligation_1 x
-                                   (exist (fun _ : ST => True) x0 preA_st0)
-                               with
-                               | ex_intro x1 H0 =>
-                                   ex_intro
-                                     (fun st0 : ST =>
-                                      exists (an : nat) 
-                                      (stA : ST),
-                                        x0 = st0 /\ an = 0 /\ stA = st0) x0
-                                     (ex_intro
-                                        (fun an : nat =>
-                                         exists stA : ST,
-                                           x0 = x0 /\ an = 0 /\ stA = x0) x1
-                                        (ex_intro
-                                           (fun stA : ST =>
-                                            x0 = x0 /\ x1 = 0 /\ stA = x0) x0
-                                           H0))
-                               end
-                               (exist (fun st : ST => st = x0) x0 preA_st1)))) in
-                  fun
-                    postA_stA : exists an : nat,
-                                  av = bare_list_insert x x0 /\
-                                  an = length x0 /\ stA = x0 =>
-                  exist
-                    (fun anonymous : () * ST =>
-                     let (_, st') := anonymous in
-                     exists (an : nat) (a0 : ST) (an0 : nat) 
-                     (stA0 : ST),
-                       (a0 = bare_list_insert x x0 /\
-                        an0 = length x0 /\ stA0 = x0) /\
-                       a0 = bare_list_insert x stA0 /\
-                       an = length stA0 /\ st' = a0) 
-                    ((), av)
-                    match postA_stA with
-                    | ex_intro an postA_stA0 =>
-                        match
-                          insert_obligation_5 x x0
-                            match
-                              insert_obligation_1 x
-                                (exist (fun _ : ST => True) x0 preA_st0)
-                            with
-                            | ex_intro x1 H0 =>
-                                ex_intro
-                                  (fun st0 : ST =>
-                                   exists (an0 : nat) 
-                                   (stA0 : ST),
-                                     x0 = st0 /\ an0 = 0 /\ stA0 = st0) x0
-                                  (ex_intro
-                                     (fun an0 : nat =>
-                                      exists stA0 : ST,
-                                        x0 = x0 /\ an0 = 0 /\ stA0 = x0) x1
-                                     (ex_intro
-                                        (fun stA0 : ST =>
-                                         x0 = x0 /\ x1 = 0 /\ stA0 = x0) x0
-                                        H0))
-                            end av
-                            match postA_stA with
-                            | ex_intro x1 H0 =>
-                                ex_intro
-                                  (fun st0 : ST =>
-                                   exists (an0 : nat) 
-                                   (stA0 : ST),
-                                     av = bare_list_insert x st0 /\
-                                     an0 = length st0 /\ stA0 = st0) x0
-                                  (ex_intro
-                                     (fun an0 : nat =>
-                                      exists stA0 : ST,
-                                        av = bare_list_insert x x0 /\
-                                        an0 = length x0 /\ stA0 = x0) x1
-                                     (ex_intro
-                                        (fun stA0 : ST =>
-                                         av = bare_list_insert x x0 /\
-                                         x1 = length x0 /\ stA0 = x0) stA H0))
-                            end
-                            (exist
-                               (fun st : ST => av = bare_list_insert x st)
-                               stA
-                               match postA_stA with
-                               | ex_intro x1 H0 => postApreB0 av x1 stA H0
-                               end)
-                        with
-                        | ex_intro bn postApostB_stB =>
-                            ex_intro
-                              (fun an0 : nat =>
-                               exists (a : ST) (an1 : nat) 
-                               (stA0 : ST),
-                                 (a = bare_list_insert x x0 /\
-                                  an1 = length x0 /\ stA0 = x0) /\
-                                 a = bare_list_insert x stA0 /\
-                                 an0 = length stA0 /\ av = a) 
-                              (an + bn)
-                              (ex_intro
-                                 (fun a : ST =>
-                                  exists (an0 : nat) 
-                                  (stA0 : ST),
-                                    (a = bare_list_insert x x0 /\
-                                     an0 = length x0 /\ stA0 = x0) /\
-                                    a = bare_list_insert x stA0 /\
-                                    an + bn = length stA0 /\ av = a) av
-                                 (ex_intro
-                                    (fun an0 : nat =>
-                                     exists stA0 : ST,
-                                       (av = bare_list_insert x x0 /\
-                                        an0 = length x0 /\ stA0 = x0) /\
-                                       av = bare_list_insert x stA0 /\
-                                       an + bn = length stA0 /\ av = av) an
-                                    (ex_intro
-                                       (fun stA0 : ST =>
-                                        (av = bare_list_insert x x0 /\
-                                         an = length x0 /\ stA0 = x0) /\
-                                        av = bare_list_insert x stA0 /\
-                                        an + bn = length stA0 /\ av = av) stA
-                                       (conj postA_stA0
-                                          (postApostB_stB x0 an postA_stA0)))))
-                        end
-                    end)
-                   (insert_obligation_3 x x0
-                      match
-                        insert_obligation_1 x
-                          (exist (fun _ : ST => True) x0 preA_st0)
-                      with
-                      | ex_intro x1 H0 =>
-                          ex_intro
-                            (fun st0 : ST =>
-                             exists (an : nat) (stA : ST),
-                               x0 = st0 /\ an = 0 /\ stA = st0) x0
-                            (ex_intro
-                               (fun an : nat =>
-                                exists stA : ST,
-                                  x0 = x0 /\ an = 0 /\ stA = x0) x1
-                               (ex_intro
-                                  (fun stA : ST =>
-                                   x0 = x0 /\ x1 = 0 /\ stA = x0) x0 H0))
-                      end (exist (fun st : ST => st = x0) x0 preA_st1))
-             end in
-         fun
-           postApostB_stB : exists an : nat,
-                              forall (st0 : ST) (an0 : nat),
-                              x0 = st0 /\ an0 = 0 /\ x0 = st0 ->
-                              x0 = x0 /\
-                              an0 + an = length x0 /\
-                              stB = bare_list_insert x x0 =>
-         exist
-           (fun anonymous : () * ST =>
-            let (_, st') := anonymous in
-            exists (an : nat) (a0 : ST) (an0 : nat) 
-            (stA : ST),
-              (a0 = x0 /\ an0 = 0 /\ stA = x0) /\
-              stA = a0 /\ an = length stA /\ st' = bare_list_insert x stA)
-           (bv, stB)
-           match
-             insert_obligation_1 x (exist (fun _ : ST => True) x0 preA_st0)
-           with
-           | ex_intro an postA_stA =>
-               match postApostB_stB with
-               | ex_intro bn postApostB_stB0 =>
-                   ex_intro
-                     (fun an0 : nat =>
-                      exists (a : ST) (an1 : nat) (stA : ST),
-                        (a = x0 /\ an1 = 0 /\ stA = x0) /\
-                        stA = a /\
-                        an0 = length stA /\ stB = bare_list_insert x stA)
-                     (an + bn)
-                     (ex_intro
-                        (fun a : ST =>
-                         exists (an0 : nat) (stA : ST),
-                           (a = x0 /\ an0 = 0 /\ stA = x0) /\
-                           stA = a /\
-                           an + bn = length stA /\
-                           stB = bare_list_insert x stA) x0
-                        (ex_intro
-                           (fun an0 : nat =>
-                            exists stA : ST,
-                              (x0 = x0 /\ an0 = 0 /\ stA = x0) /\
-                              stA = x0 /\
-                              an + bn = length stA /\
-                              stB = bare_list_insert x stA) an
-                           (ex_intro
-                              (fun stA : ST =>
-                               (x0 = x0 /\ an = 0 /\ stA = x0) /\
-                               stA = x0 /\
-                               an + bn = length stA /\
-                               stB = bare_list_insert x stA) x0
-                              (conj postA_stA
-                                 (postApostB_stB0 x0 an postA_stA)))))
-               end
-           end) y).
-  
-  destruct (insert_obligation_6 x x0
-              match
-                insert_obligation_1 x
-                  (exist (fun _ : ST => True) x0 preA_st0)
-              with
-              | ex_intro x1 H0 =>
-                  ex_intro
-                    (fun st0 : ST =>
-                     exists (an : nat) (stA : ST),
-                       x0 = st0 /\ an = 0 /\ stA = st0) x0
-                    (ex_intro
-                       (fun an : nat =>
-                        exists stA : ST, x0 = x0 /\ an = 0 /\ stA = x0) x1
-                       (ex_intro
-                          (fun stA : ST => x0 = x0 /\ x1 = 0 /\ stA = x0) x0
-                          H0))
-              end
-              (exist (fun st : ST => st = x0) x0
-                 match
-                   insert_obligation_1 x
-                     (exist (fun _ : ST => True) x0 preA_st0)
-                 with
-                 | ex_intro x1 H0 => postApreB x0 x1 x0 H0
-                 end))
-  as [preA_st1 postApreB0].
-  simpl in *.
-  
-  clear y.
-
-program_simpl.
-  
-  simpl in *.  
-  remember (insert_obligation_7 x x0
-             (ex_intro
-                (fun st0 : ST =>
-                 exists (an : nat) (stA : ST),
-                   x0 = st0 /\ an = 0 /\ stA = st0) x0
-                (ex_intro
-                   (fun an : nat =>
-                    exists stA : ST, x0 = x0 /\ an = 0 /\ stA = x0) x1
-                   (ex_intro (fun stA : ST => x0 = x0 /\ x1 = 0 /\ stA = x0)
-                      x0 a)))
-             (exist (fun st : ST => st = x0) x0 (e x0 x1 x0 a))).
-  simpl in *.
-  
-  
-  eauto.
-  
-  exists (length postl).
-  destruct (list_insert x postl (exist (fun _ : ST => True) postl I))
-    as [[a st'] [an [EQa [EQan EQst']]]].
-  
-  eauto.
-  split. auto.
-  
-  eauto.
+  (* 1277 lines! *)
+Admitted.
 
 End dumb_list.
+
+Extract Inductive unit => "unit" [ "tt" ].
+Extract Inductive bool => "bool" [ "false" "true" ].
+Extract Inductive sumbool => "bool" [ "false" "true" ].
+Extract Inductive prod => "(*)"  [ "(,)" ].
+Extract Inductive nat => 
+"int" [ "0" "succ" ]
+      "(fun fO fS n -> if n=0 then fO () else fS (n-1))".
+
+Extract Constant plus => "fun x y -> x + y".
+Extract Constant mult => "fun x y -> x * y".
+Extract Constant minus => "fun x y -> x - y".
+
+Extraction Inline ret bind inc get put.
+Extraction Inline projT1 projT2.
 
 Recursive Extraction insert.
